# XM531 Problem Set 4 (Quang Doan)


## Problem 1 

The `gamma function` is denoted by $\Gamma(p)$ and is defined by the integral

$$\Gamma(p+1)=\int_0^\infty e^{-x}x^pdx $$

**A.** Show that, for $p>0, \Gamma(p+1) = p\Gamma(p)$

By definition

$$\Gamma(p) = \int_0^\infty e^{-x}x^{p-1}dx$$

Thus,

$$p \Gamma(p) = p \int_0^\infty e^{-x}x^{p-1}dx = \int_0^\infty e^{-x} p x^{p-1}dx$$

we need to show that 

$$\Gamma(p+1)=\int_0^\infty e^{-x}x^pdx = \int_0^\infty e^{-x} p x^{p-1}dx \quad (*) $$

Let

$$u = x^p, \quad  du = p x^{p-1} dx $$
$$dv = e^{-x}dx,  v = -e^{-x} $$


$$\int e^{-x}x^pdx \quad \text{is} \int udv = uv - \int vdu $$ 


$$\int_0^\infty e^{-x}x^pdx = -x^p e^{-x} |_0^{\infty} -  \int_0^\infty -e^{-x} p x^{p-1} dx 
= (0 - 0) + \int_0^\infty e^{-x} p x^{p-1} dx = \int_0^\infty e^{-x} p x^{p-1} dx $$ 

Thus 

$$\Gamma(p+1)=\int_0^\infty e^{-x}x^pdx = \int_0^\infty e^{-x} p x^{p-1}dx 
 = p \int_0^\infty e^{-x}x^{p-1}dx = p \Gamma(p) \quad  \text{Q.E.D.}$$



**B.** Show that $\Gamma(1)=1$

By definition

$$\Gamma(1) = \int_0^\infty e^{-x}x^{0}dx 
= \int_0^\infty e^{-x}dx $$

$$\Gamma(1) = \int_0^\infty e^{-x}dx = -e^{-x}|_0^\infty $$
$$\Gamma(1) = -e^{-x}|_0^\infty = -0 - (-e^0) = e^0 = 1 $$

**C.** If $p$ is a positive integer $n$, show that $\Gamma(n+1) = n!$

Prove by induction:

Base case: $n = 1$:

$$\Gamma(1+1) = 1*\Gamma(1) \quad \text{per part A} $$
$$1*\Gamma(1) = 1*1 \quad \text{per part B} $$
$$\Gamma(n+1) = \Gamma(1+1) = 1 = n! \quad \text{for n = 1}  $$

Induction step:

- Suppose that for some positive integer $k$ 
$$\Gamma(k+1) = k!  $$

- we must show that 

$$\Gamma(k+2) = (k+1)!  $$

- Applying the result from part **A**:   $\Gamma(p+1) = p\Gamma(p)$, with p = (k+1) 

$$\Gamma(k+2) = \Gamma( \mathbf{(k+1)} + 1 ) = (k+1) \Gamma(k+1) $$
$$(k+1) \Gamma(k+1) = (k+1) k!  \quad \text{per induction hypothesis} $$

$$\text{thus} \quad \Gamma(k+2) = (k+1) k! = (k+1)!$$

we have shown that 

$$\Gamma(n+1) = n! \quad \text{by induction}$$



**D.** Show that, for $p>0$, 

$$p(p+1)(p+2)\dots (p+n-1) = \frac{\Gamma(p+n)}{\Gamma(p)} $$ 


Applying the result from part **A**

- $\Gamma(p+1) =  (p) \Gamma(p)$
- $\Gamma(p+2) = (p+1) \Gamma( p+1) = (p+1) (p) \Gamma( p) $
- $\Gamma(p+3) = (p+2) \Gamma( p+2) = (p+2) (p+1) (p) \Gamma( p) $
- ...
- $\Gamma(p+n) = (p + n - 1) (p + n - 2) \cdot \cdot \cdot (p+1) (p) \Gamma( p) $

Thus 

$$p(p+1)(p+2)\dots (p+n-1) = \frac{\Gamma(p+n)}{\Gamma(p)} $$ 

**E.** Given $\Gamma(\frac{1}{2}) = \sqrt \pi$, find $\Gamma(\frac{3}{2})$, and $\Gamma(\frac{11}{2})$


$$\Gamma(\frac{3}{2})=\Gamma(\frac{1}{2} + 1)=\frac{1}{2} \cdot \Gamma(\frac{1}{2})=\frac{\sqrt \pi}{2}$$ 

$$\Gamma(\frac{11}{2})=\Gamma(\frac{1}{2} + 5) = 
\frac{1}{2} \cdot 
\frac{3}{2} \cdot 
\frac{5}{2} \cdot 
\frac{7}{2} \cdot 
\frac{9}{2} \cdot 
\Gamma(\frac{1}{2})$$ 


$$\Gamma(\frac{11}{2}) = 
\frac{1 \cdot 3 \cdot 5 \cdot 7 \cdot 9}{32} \sqrt \pi = 

\frac{945}{32} \sqrt \pi = 52.36 


$$ 
